# baseURI: http://onto.fel.cvut.cz/ontologies/form-spin

@prefix : <http://onto.fel.cvut.cz/ontologies/form-spin/> .
@prefix dc: <http://purl.org/dc/elements/1.1/> .
@prefix doc: <http://onto.fel.cvut.cz/ontologies/documentation/> .
@prefix form: <http://onto.fel.cvut.cz/ontologies/form/> .
@prefix owl: <http://www.w3.org/2002/07/owl#> .
@prefix rdf: <http://www.w3.org/1999/02/22-rdf-syntax-ns#> .
@prefix rdfs: <http://www.w3.org/2000/01/rdf-schema#> .
@prefix xml: <http://www.w3.org/XML/1998/namespace> .
@prefix xsd: <http://www.w3.org/2001/XMLSchema#> .
@prefix sh:   <http://www.w3.org/ns/shacl#> .

<http://onto.fel.cvut.cz/ontologies/form-spin>
  rdf:type owl:Ontology ;
  rdfs:comment "Represent form answer types that are represented as string literal with restriction to a grammar e.g. textual representation of SPARQL queries and SPARQL expressions." ;
.

:has-answer-value-type
  rdf:type owl:ObjectProperty ;
  rdfs:comment "Represents a type of answer values based on the question" ;
  rdfs:domain doc:question ;
  rdfs:label "has answer value type" ;
.

:has-origin-context
  rdf:type owl:ObjectProperty ;
  rdfs:comment "Represents the context IRI where the question's origin comes from." ;
  rdfs:domain doc:question ;
  rdfs:label "has origin context" ;
.


:has-declared-prefix
    rdf:type owl:ObjectProperty ;
    rdfs:comment "Represents an declared prefix that can be used within SPARQL query of an answer of this question." ;
    rdfs:domain doc:question ;
    rdfs:range sh:PrefixDeclaration ;
.


sh:PrefixDeclaration
	a rdfs:Class ;
	rdfs:label "Prefix declaration"@en ;
	rdfs:comment "The class of prefix declarations, consisting of pairs of a prefix with a namespace."@en ;
	rdfs:subClassOf rdfs:Resource ;
	rdfs:isDefinedBy sh: ;
.

sh:prefix
	a rdf:Property ;
	rdfs:label "prefix"@en ;
	rdfs:comment "The prefix of a prefix declaration."@en ;
	rdfs:domain sh:PrefixDeclaration ;
	rdfs:range xsd:string ;
	rdfs:isDefinedBy sh: ;
.

sh:namespace
	a rdf:Property ;
	rdfs:label "namespace"@en ;
	rdfs:comment "The namespace associated with a prefix in a prefix declaration."@en ;
	rdfs:domain sh:PrefixDeclaration ;
	rdfs:range xsd:anyURI ;
	rdfs:isDefinedBy sh: ;
.